...

Risc0/Gadgets/OneHot20/Witness/WeakestPresPart16.lean
@@ -10,90 +10,96 @@ open MLIRNotation
 -- The state obtained by running Code.part16 on st
 def part16_state (st: State) : State :=
   
-          ((((State.set! st { name := "data" } 6 (Option.get! st.felts[({ name := "%102" }: FeltVar)]!))["%20"] ←ₛ
-                getImpl (State.set! st { name := "data" } 6 (Option.get! st.felts[({ name := "%102" }: FeltVar)]!))
-                  { name := "in" } 0 0)[felts][{ name := "%103" }] ←
-              feltBitAnd
-                (Option.get!
-                  (State.felts
-                    ((State.set! st { name := "data" } 6 (Option.get! st.felts[({ name := "%102" }: FeltVar)]!))["%20"] ←ₛ
-                      getImpl (State.set! st { name := "data" } 6 (Option.get! st.felts[({ name := "%102" }: FeltVar)]!))
-                        { name := "in" } 0 0)
-                    { name := "%20" }))
-                (Option.get! (State.felts st { name := "%19" })))[felts][{ name := "%104" }] ←
-            feltBitAnd
-                (Option.get!
-                  (State.felts
-                    ((State.set! st { name := "data" } 6 (Option.get! st.felts[({ name := "%102" }: FeltVar)]!))["%20"] ←ₛ
-                      getImpl (State.set! st { name := "data" } 6 (Option.get! st.felts[({ name := "%102" }: FeltVar)]!))
-                        { name := "in" } 0 0)
-                    { name := "%20" }))
-                (Option.get! (State.felts st { name := "%19" })) *
-              Option.get! (State.felts st { name := "%18" })) 
+          ((State.set!
+              ((st[felts][{ name := "%169" }] ←
+                  Option.get! (State.felts st { name := "%20" }) -
+                    Option.get! (State.felts st { name := "%3" }))[felts][{ name := "%170" }] ←
+                if
+                    Option.get! (State.felts st { name := "%20" }) - Option.get! (State.felts st { name := "%3" }) =
+                      0 then
+                  1
+                else 0)
+              { name := "data" } 16
+              (if
+                  Option.get! (State.felts st { name := "%20" }) - Option.get! (State.felts st { name := "%3" }) =
+                    0 then
+                1
+              else 0))[felts][{ name := "%2" }] ←
+            17) 
 
 def part16_drops (st: State) : State :=
-  State.dropFelts (State.dropFelts (State.dropFelts (st) ⟨"%18"⟩) ⟨"%102"⟩) ⟨"%103"⟩
+  State.dropFelts (State.dropFelts (st) ⟨"%169"⟩) ⟨"%170"⟩
 
 -- Run the program from part16 onwards by using part16_state rather than Code.part16
 def part16_state_update (st: State): State :=
-  Γ (part16_drops (part16_state st)) ⟦Code.part17;dropfelt ⟨"%104"⟩;dropfelt ⟨"%0"⟩;dropfelt ⟨"%105"⟩;Code.part18;dropfelt ⟨"%26"⟩;Code.part19;dropfelt ⟨"%28"⟩;dropfelt ⟨"%29"⟩;dropfelt ⟨"%30"⟩;dropfelt ⟨"%31"⟩;Code.part20;dropfelt ⟨"%27"⟩;dropfelt ⟨"%32"⟩;dropfelt ⟨"%33"⟩;dropfelt ⟨"%25"⟩;Code.part21;dropfelt ⟨"%3"⟩;dropfelt ⟨"%34"⟩;dropfelt ⟨"%35"⟩;dropfelt ⟨"%36"⟩;dropfelt ⟨"%37"⟩;Code.part22;dropfelt ⟨"%23"⟩;dropfelt ⟨"%38"⟩;dropfelt ⟨"%24"⟩;dropfelt ⟨"%39"⟩;dropfelt ⟨"%40"⟩;Code.part23;dropfelt ⟨"%11"⟩;dropfelt ⟨"%42"⟩;dropfelt ⟨"%45"⟩;Code.part24;dropfelt ⟨"%13"⟩;dropfelt ⟨"%46"⟩;dropfelt ⟨"%47"⟩;dropfelt ⟨"%48"⟩;Code.part25;dropfelt ⟨"%43"⟩;dropfelt ⟨"%49"⟩;dropfelt ⟨"%44"⟩;dropfelt ⟨"%50"⟩;dropfelt ⟨"%51"⟩;Code.part26;dropfelt ⟨"%22"⟩;dropfelt ⟨"%52"⟩;dropfelt ⟨"%41"⟩;dropfelt ⟨"%53"⟩;dropfelt ⟨"%54"⟩;Code.part27;dropfelt ⟨"%7"⟩;dropfelt ⟨"%56"⟩;dropfelt ⟨"%59"⟩;Code.part28;dropfelt ⟨"%15"⟩;dropfelt ⟨"%60"⟩;dropfelt ⟨"%58"⟩;dropfelt ⟨"%61"⟩;dropfelt ⟨"%63"⟩;Code.part29;dropfelt ⟨"%57"⟩;dropfelt ⟨"%62"⟩;dropfelt ⟨"%64"⟩;dropfelt ⟨"%65"⟩;dropfelt ⟨"%66"⟩;dropfelt ⟨"%55"⟩;Code.part30;dropfelt ⟨"%19"⟩;dropfelt ⟨"%21"⟩;dropfelt ⟨"%67"⟩;dropfelt ⟨"%68"⟩;dropfelt ⟨"%70"⟩;Code.part31;dropfelt ⟨"%20"⟩;dropfelt ⟨"%71"⟩;dropfelt ⟨"%69"⟩;dropfelt ⟨"%72"⟩;dropfelt ⟨"%73"⟩⟧
+  Γ (part16_drops (part16_state st)) ⟦Code.part17;dropfelt ⟨"%171"⟩;dropfelt ⟨"%172"⟩;Code.part18;dropfelt ⟨"%173"⟩;dropfelt ⟨"%174"⟩;Code.part19;dropfelt ⟨"%175"⟩;dropfelt ⟨"%176"⟩;Code.part20;dropfelt ⟨"%17"⟩;dropfelt ⟨"%23"⟩;Code.part21;dropfelt ⟨"%16"⟩;dropfelt ⟨"%15"⟩;dropfelt ⟨"%24"⟩;dropfelt ⟨"%26"⟩;Code.part22;dropfelt ⟨"%14"⟩;dropfelt ⟨"%27"⟩;dropfelt ⟨"%29"⟩;dropfelt ⟨"%30"⟩;dropfelt ⟨"%32"⟩;Code.part23;dropfelt ⟨"%13"⟩;dropfelt ⟨"%33"⟩;dropfelt ⟨"%35"⟩;Code.part24;dropfelt ⟨"%12"⟩;dropfelt ⟨"%11"⟩;dropfelt ⟨"%36"⟩;dropfelt ⟨"%38"⟩;Code.part25;dropfelt ⟨"%10"⟩;dropfelt ⟨"%39"⟩;dropfelt ⟨"%41"⟩;dropfelt ⟨"%42"⟩;dropfelt ⟨"%44"⟩;Code.part26;dropfelt ⟨"%9"⟩;dropfelt ⟨"%45"⟩;dropfelt ⟨"%47"⟩;Code.part27;dropfelt ⟨"%8"⟩;dropfelt ⟨"%7"⟩;dropfelt ⟨"%48"⟩;dropfelt ⟨"%50"⟩;Code.part28;dropfelt ⟨"%6"⟩;dropfelt ⟨"%51"⟩;dropfelt ⟨"%53"⟩;dropfelt ⟨"%54"⟩;dropfelt ⟨"%56"⟩;Code.part29;dropfelt ⟨"%5"⟩;dropfelt ⟨"%57"⟩;dropfelt ⟨"%59"⟩;Code.part30;dropfelt ⟨"%4"⟩;dropfelt ⟨"%3"⟩;dropfelt ⟨"%60"⟩;dropfelt ⟨"%62"⟩;Code.part31;dropfelt ⟨"%2"⟩;dropfelt ⟨"%63"⟩;dropfelt ⟨"%65"⟩;dropfelt ⟨"%66"⟩;dropfelt ⟨"%68"⟩;Code.part32;dropfelt ⟨"%1"⟩;dropfelt ⟨"%69"⟩;dropfelt ⟨"%71"⟩;Code.part33;dropfelt ⟨"%20"⟩;dropfelt ⟨"%0"⟩;dropfelt ⟨"%72"⟩;dropfelt ⟨"%74"⟩;dropfelt ⟨"%75"⟩;dropfelt ⟨"%76"⟩;Code.part34;dropfelt ⟨"%78"⟩;dropfelt ⟨"%79"⟩;Code.part35;dropfelt ⟨"%21"⟩;dropfelt ⟨"%77"⟩;dropfelt ⟨"%80"⟩;dropfelt ⟨"%81"⟩;Code.part36;dropfelt ⟨"%22"⟩;dropfelt ⟨"%82"⟩;dropfelt ⟨"%83"⟩;dropfelt ⟨"%84"⟩;Code.part37;dropfelt ⟨"%25"⟩;dropfelt ⟨"%85"⟩;dropfelt ⟨"%86"⟩;dropfelt ⟨"%87"⟩;Code.part38;dropfelt ⟨"%28"⟩;dropfelt ⟨"%88"⟩;dropfelt ⟨"%89"⟩;dropfelt ⟨"%90"⟩;Code.part39;dropfelt ⟨"%31"⟩;dropfelt ⟨"%91"⟩;dropfelt ⟨"%92"⟩;dropfelt ⟨"%93"⟩;Code.part40;dropfelt ⟨"%34"⟩;dropfelt ⟨"%94"⟩;dropfelt ⟨"%95"⟩;dropfelt ⟨"%96"⟩;Code.part41;dropfelt ⟨"%37"⟩;dropfelt ⟨"%97"⟩;dropfelt ⟨"%98"⟩;dropfelt ⟨"%99"⟩;Code.part42;dropfelt ⟨"%40"⟩;dropfelt ⟨"%100"⟩;dropfelt ⟨"%101"⟩;dropfelt ⟨"%102"⟩;Code.part43;dropfelt ⟨"%43"⟩;dropfelt ⟨"%103"⟩;dropfelt ⟨"%104"⟩;dropfelt ⟨"%105"⟩;Code.part44;dropfelt ⟨"%46"⟩;dropfelt ⟨"%106"⟩;dropfelt ⟨"%107"⟩;dropfelt ⟨"%108"⟩;Code.part45;dropfelt ⟨"%49"⟩;dropfelt ⟨"%109"⟩;dropfelt ⟨"%110"⟩;dropfelt ⟨"%111"⟩;Code.part46;dropfelt ⟨"%52"⟩;dropfelt ⟨"%112"⟩;dropfelt ⟨"%113"⟩;dropfelt ⟨"%114"⟩;Code.part47;dropfelt ⟨"%55"⟩;dropfelt ⟨"%115"⟩;dropfelt ⟨"%116"⟩;dropfelt ⟨"%117"⟩;Code.part48;dropfelt ⟨"%58"⟩;dropfelt ⟨"%118"⟩;dropfelt ⟨"%119"⟩;dropfelt ⟨"%120"⟩;Code.part49;dropfelt ⟨"%61"⟩;dropfelt ⟨"%121"⟩;dropfelt ⟨"%122"⟩;dropfelt ⟨"%123"⟩;Code.part50;dropfelt ⟨"%64"⟩;dropfelt ⟨"%124"⟩;dropfelt ⟨"%125"⟩;dropfelt ⟨"%126"⟩;Code.part51;dropfelt ⟨"%67"⟩;dropfelt ⟨"%127"⟩;dropfelt ⟨"%128"⟩;dropfelt ⟨"%129"⟩;Code.part52;dropfelt ⟨"%70"⟩;dropfelt ⟨"%130"⟩;dropfelt ⟨"%131"⟩;dropfelt ⟨"%132"⟩;Code.part53;dropfelt ⟨"%73"⟩;dropfelt ⟨"%133"⟩;dropfelt ⟨"%134"⟩;dropfelt ⟨"%135"⟩;Code.part54;dropfelt ⟨"%18"⟩;dropfelt ⟨"%136"⟩;dropfelt ⟨"%137"⟩;dropfelt ⟨"%19"⟩⟧
 
 -- Prove that substituting part16_state for Code.part16 produces the same result
-lemma part16_wp {st : State} {y0 y1 y2 y3 y4 y5 y6 y7 y8 y9 y10 y11 y12 y13 y14 y15 y16 y17 : Option Felt} :
-  Code.getReturn (MLIR.runProgram (Code.part16;dropfelt ⟨"%18"⟩;dropfelt ⟨"%102"⟩;dropfelt ⟨"%103"⟩;Code.part17;dropfelt ⟨"%104"⟩;dropfelt ⟨"%0"⟩;dropfelt ⟨"%105"⟩;Code.part18;dropfelt ⟨"%26"⟩;Code.part19;dropfelt ⟨"%28"⟩;dropfelt ⟨"%29"⟩;dropfelt ⟨"%30"⟩;dropfelt ⟨"%31"⟩;Code.part20;dropfelt ⟨"%27"⟩;dropfelt ⟨"%32"⟩;dropfelt ⟨"%33"⟩;dropfelt ⟨"%25"⟩;Code.part21;dropfelt ⟨"%3"⟩;dropfelt ⟨"%34"⟩;dropfelt ⟨"%35"⟩;dropfelt ⟨"%36"⟩;dropfelt ⟨"%37"⟩;Code.part22;dropfelt ⟨"%23"⟩;dropfelt ⟨"%38"⟩;dropfelt ⟨"%24"⟩;dropfelt ⟨"%39"⟩;dropfelt ⟨"%40"⟩;Code.part23;dropfelt ⟨"%11"⟩;dropfelt ⟨"%42"⟩;dropfelt ⟨"%45"⟩;Code.part24;dropfelt ⟨"%13"⟩;dropfelt ⟨"%46"⟩;dropfelt ⟨"%47"⟩;dropfelt ⟨"%48"⟩;Code.part25;dropfelt ⟨"%43"⟩;dropfelt ⟨"%49"⟩;dropfelt ⟨"%44"⟩;dropfelt ⟨"%50"⟩;dropfelt ⟨"%51"⟩;Code.part26;dropfelt ⟨"%22"⟩;dropfelt ⟨"%52"⟩;dropfelt ⟨"%41"⟩;dropfelt ⟨"%53"⟩;dropfelt ⟨"%54"⟩;Code.part27;dropfelt ⟨"%7"⟩;dropfelt ⟨"%56"⟩;dropfelt ⟨"%59"⟩;Code.part28;dropfelt ⟨"%15"⟩;dropfelt ⟨"%60"⟩;dropfelt ⟨"%58"⟩;dropfelt ⟨"%61"⟩;dropfelt ⟨"%63"⟩;Code.part29;dropfelt ⟨"%57"⟩;dropfelt ⟨"%62"⟩;dropfelt ⟨"%64"⟩;dropfelt ⟨"%65"⟩;dropfelt ⟨"%66"⟩;dropfelt ⟨"%55"⟩;Code.part30;dropfelt ⟨"%19"⟩;dropfelt ⟨"%21"⟩;dropfelt ⟨"%67"⟩;dropfelt ⟨"%68"⟩;dropfelt ⟨"%70"⟩;Code.part31;dropfelt ⟨"%20"⟩;dropfelt ⟨"%71"⟩;dropfelt ⟨"%69"⟩;dropfelt ⟨"%72"⟩;dropfelt ⟨"%73"⟩) st) = [y0, y1, y2, y3, y4, y5, y6, y7, y8, y9, y10, y11, y12, y13, y14, y15, y16, y17] ↔
-  Code.getReturn (part16_state_update st) = [y0, y1, y2, y3, y4, y5, y6, y7, y8, y9, y10, y11, y12, y13, y14, y15, y16, y17] := by
+lemma part16_wp {st : State} {y0 y1 y2 y3 y4 y5 y6 y7 y8 y9 y10 y11 y12 y13 y14 y15 y16 y17 y18 y19 : Option Felt} :
+  Code.getReturn (MLIR.runProgram (Code.part16;dropfelt ⟨"%169"⟩;dropfelt ⟨"%170"⟩;Code.part17;dropfelt ⟨"%171"⟩;dropfelt ⟨"%172"⟩;Code.part18;dropfelt ⟨"%173"⟩;dropfelt ⟨"%174"⟩;Code.part19;dropfelt ⟨"%175"⟩;dropfelt ⟨"%176"⟩;Code.part20;dropfelt ⟨"%17"⟩;dropfelt ⟨"%23"⟩;Code.part21;dropfelt ⟨"%16"⟩;dropfelt ⟨"%15"⟩;dropfelt ⟨"%24"⟩;dropfelt ⟨"%26"⟩;Code.part22;dropfelt ⟨"%14"⟩;dropfelt ⟨"%27"⟩;dropfelt ⟨"%29"⟩;dropfelt ⟨"%30"⟩;dropfelt ⟨"%32"⟩;Code.part23;dropfelt ⟨"%13"⟩;dropfelt ⟨"%33"⟩;dropfelt ⟨"%35"⟩;Code.part24;dropfelt ⟨"%12"⟩;dropfelt ⟨"%11"⟩;dropfelt ⟨"%36"⟩;dropfelt ⟨"%38"⟩;Code.part25;dropfelt ⟨"%10"⟩;dropfelt ⟨"%39"⟩;dropfelt ⟨"%41"⟩;dropfelt ⟨"%42"⟩;dropfelt ⟨"%44"⟩;Code.part26;dropfelt ⟨"%9"⟩;dropfelt ⟨"%45"⟩;dropfelt ⟨"%47"⟩;Code.part27;dropfelt ⟨"%8"⟩;dropfelt ⟨"%7"⟩;dropfelt ⟨"%48"⟩;dropfelt ⟨"%50"⟩;Code.part28;dropfelt ⟨"%6"⟩;dropfelt ⟨"%51"⟩;dropfelt ⟨"%53"⟩;dropfelt ⟨"%54"⟩;dropfelt ⟨"%56"⟩;Code.part29;dropfelt ⟨"%5"⟩;dropfelt ⟨"%57"⟩;dropfelt ⟨"%59"⟩;Code.part30;dropfelt ⟨"%4"⟩;dropfelt ⟨"%3"⟩;dropfelt ⟨"%60"⟩;dropfelt ⟨"%62"⟩;Code.part31;dropfelt ⟨"%2"⟩;dropfelt ⟨"%63"⟩;dropfelt ⟨"%65"⟩;dropfelt ⟨"%66"⟩;dropfelt ⟨"%68"⟩;Code.part32;dropfelt ⟨"%1"⟩;dropfelt ⟨"%69"⟩;dropfelt ⟨"%71"⟩;Code.part33;dropfelt ⟨"%20"⟩;dropfelt ⟨"%0"⟩;dropfelt ⟨"%72"⟩;dropfelt ⟨"%74"⟩;dropfelt ⟨"%75"⟩;dropfelt ⟨"%76"⟩;Code.part34;dropfelt ⟨"%78"⟩;dropfelt ⟨"%79"⟩;Code.part35;dropfelt ⟨"%21"⟩;dropfelt ⟨"%77"⟩;dropfelt ⟨"%80"⟩;dropfelt ⟨"%81"⟩;Code.part36;dropfelt ⟨"%22"⟩;dropfelt ⟨"%82"⟩;dropfelt ⟨"%83"⟩;dropfelt ⟨"%84"⟩;Code.part37;dropfelt ⟨"%25"⟩;dropfelt ⟨"%85"⟩;dropfelt ⟨"%86"⟩;dropfelt ⟨"%87"⟩;Code.part38;dropfelt ⟨"%28"⟩;dropfelt ⟨"%88"⟩;dropfelt ⟨"%89"⟩;dropfelt ⟨"%90"⟩;Code.part39;dropfelt ⟨"%31"⟩;dropfelt ⟨"%91"⟩;dropfelt ⟨"%92"⟩;dropfelt ⟨"%93"⟩;Code.part40;dropfelt ⟨"%34"⟩;dropfelt ⟨"%94"⟩;dropfelt ⟨"%95"⟩;dropfelt ⟨"%96"⟩;Code.part41;dropfelt ⟨"%37"⟩;dropfelt ⟨"%97"⟩;dropfelt ⟨"%98"⟩;dropfelt ⟨"%99"⟩;Code.part42;dropfelt ⟨"%40"⟩;dropfelt ⟨"%100"⟩;dropfelt ⟨"%101"⟩;dropfelt ⟨"%102"⟩;Code.part43;dropfelt ⟨"%43"⟩;dropfelt ⟨"%103"⟩;dropfelt ⟨"%104"⟩;dropfelt ⟨"%105"⟩;Code.part44;dropfelt ⟨"%46"⟩;dropfelt ⟨"%106"⟩;dropfelt ⟨"%107"⟩;dropfelt ⟨"%108"⟩;Code.part45;dropfelt ⟨"%49"⟩;dropfelt ⟨"%109"⟩;dropfelt ⟨"%110"⟩;dropfelt ⟨"%111"⟩;Code.part46;dropfelt ⟨"%52"⟩;dropfelt ⟨"%112"⟩;dropfelt ⟨"%113"⟩;dropfelt ⟨"%114"⟩;Code.part47;dropfelt ⟨"%55"⟩;dropfelt ⟨"%115"⟩;dropfelt ⟨"%116"⟩;dropfelt ⟨"%117"⟩;Code.part48;dropfelt ⟨"%58"⟩;dropfelt ⟨"%118"⟩;dropfelt ⟨"%119"⟩;dropfelt ⟨"%120"⟩;Code.part49;dropfelt ⟨"%61"⟩;dropfelt ⟨"%121"⟩;dropfelt ⟨"%122"⟩;dropfelt ⟨"%123"⟩;Code.part50;dropfelt ⟨"%64"⟩;dropfelt ⟨"%124"⟩;dropfelt ⟨"%125"⟩;dropfelt ⟨"%126"⟩;Code.part51;dropfelt ⟨"%67"⟩;dropfelt ⟨"%127"⟩;dropfelt ⟨"%128"⟩;dropfelt ⟨"%129"⟩;Code.part52;dropfelt ⟨"%70"⟩;dropfelt ⟨"%130"⟩;dropfelt ⟨"%131"⟩;dropfelt ⟨"%132"⟩;Code.part53;dropfelt ⟨"%73"⟩;dropfelt ⟨"%133"⟩;dropfelt ⟨"%134"⟩;dropfelt ⟨"%135"⟩;Code.part54;dropfelt ⟨"%18"⟩;dropfelt ⟨"%136"⟩;dropfelt ⟨"%137"⟩;dropfelt ⟨"%19"⟩) st) = [y0, y1, y2, y3, y4, y5, y6, y7, y8, y9, y10, y11, y12, y13, y14, y15, y16, y17, y18, y19] ↔
+  Code.getReturn (part16_state_update st) = [y0, y1, y2, y3, y4, y5, y6, y7, y8, y9, y10, y11, y12, y13, y14, y15, y16, y17, y18, y19] := by
   unfold MLIR.runProgram; simp only
-  generalize eq : (dropfelt ⟨"%18"⟩;dropfelt ⟨"%102"⟩;dropfelt ⟨"%103"⟩;Code.part17;dropfelt ⟨"%104"⟩;dropfelt ⟨"%0"⟩;dropfelt ⟨"%105"⟩;Code.part18;dropfelt ⟨"%26"⟩;Code.part19;dropfelt ⟨"%28"⟩;dropfelt ⟨"%29"⟩;dropfelt ⟨"%30"⟩;dropfelt ⟨"%31"⟩;Code.part20;dropfelt ⟨"%27"⟩;dropfelt ⟨"%32"⟩;dropfelt ⟨"%33"⟩;dropfelt ⟨"%25"⟩;Code.part21;dropfelt ⟨"%3"⟩;dropfelt ⟨"%34"⟩;dropfelt ⟨"%35"⟩;dropfelt ⟨"%36"⟩;dropfelt ⟨"%37"⟩;Code.part22;dropfelt ⟨"%23"⟩;dropfelt ⟨"%38"⟩;dropfelt ⟨"%24"⟩;dropfelt ⟨"%39"⟩;dropfelt ⟨"%40"⟩;Code.part23;dropfelt ⟨"%11"⟩;dropfelt ⟨"%42"⟩;dropfelt ⟨"%45"⟩;Code.part24;dropfelt ⟨"%13"⟩;dropfelt ⟨"%46"⟩;dropfelt ⟨"%47"⟩;dropfelt ⟨"%48"⟩;Code.part25;dropfelt ⟨"%43"⟩;dropfelt ⟨"%49"⟩;dropfelt ⟨"%44"⟩;dropfelt ⟨"%50"⟩;dropfelt ⟨"%51"⟩;Code.part26;dropfelt ⟨"%22"⟩;dropfelt ⟨"%52"⟩;dropfelt ⟨"%41"⟩;dropfelt ⟨"%53"⟩;dropfelt ⟨"%54"⟩;Code.part27;dropfelt ⟨"%7"⟩;dropfelt ⟨"%56"⟩;dropfelt ⟨"%59"⟩;Code.part28;dropfelt ⟨"%15"⟩;dropfelt ⟨"%60"⟩;dropfelt ⟨"%58"⟩;dropfelt ⟨"%61"⟩;dropfelt ⟨"%63"⟩;Code.part29;dropfelt ⟨"%57"⟩;dropfelt ⟨"%62"⟩;dropfelt ⟨"%64"⟩;dropfelt ⟨"%65"⟩;dropfelt ⟨"%66"⟩;dropfelt ⟨"%55"⟩;Code.part30;dropfelt ⟨"%19"⟩;dropfelt ⟨"%21"⟩;dropfelt ⟨"%67"⟩;dropfelt ⟨"%68"⟩;dropfelt ⟨"%70"⟩;Code.part31;dropfelt ⟨"%20"⟩;dropfelt ⟨"%71"⟩;dropfelt ⟨"%69"⟩;dropfelt ⟨"%72"⟩;dropfelt ⟨"%73"⟩) = prog
+  generalize eq : (dropfelt ⟨"%169"⟩;dropfelt ⟨"%170"⟩;Code.part17;dropfelt ⟨"%171"⟩;dropfelt ⟨"%172"⟩;Code.part18;dropfelt ⟨"%173"⟩;dropfelt ⟨"%174"⟩;Code.part19;dropfelt ⟨"%175"⟩;dropfelt ⟨"%176"⟩;Code.part20;dropfelt ⟨"%17"⟩;dropfelt ⟨"%23"⟩;Code.part21;dropfelt ⟨"%16"⟩;dropfelt ⟨"%15"⟩;dropfelt ⟨"%24"⟩;dropfelt ⟨"%26"⟩;Code.part22;dropfelt ⟨"%14"⟩;dropfelt ⟨"%27"⟩;dropfelt ⟨"%29"⟩;dropfelt ⟨"%30"⟩;dropfelt ⟨"%32"⟩;Code.part23;dropfelt ⟨"%13"⟩;dropfelt ⟨"%33"⟩;dropfelt ⟨"%35"⟩;Code.part24;dropfelt ⟨"%12"⟩;dropfelt ⟨"%11"⟩;dropfelt ⟨"%36"⟩;dropfelt ⟨"%38"⟩;Code.part25;dropfelt ⟨"%10"⟩;dropfelt ⟨"%39"⟩;dropfelt ⟨"%41"⟩;dropfelt ⟨"%42"⟩;dropfelt ⟨"%44"⟩;Code.part26;dropfelt ⟨"%9"⟩;dropfelt ⟨"%45"⟩;dropfelt ⟨"%47"⟩;Code.part27;dropfelt ⟨"%8"⟩;dropfelt ⟨"%7"⟩;dropfelt ⟨"%48"⟩;dropfelt ⟨"%50"⟩;Code.part28;dropfelt ⟨"%6"⟩;dropfelt ⟨"%51"⟩;dropfelt ⟨"%53"⟩;dropfelt ⟨"%54"⟩;dropfelt ⟨"%56"⟩;Code.part29;dropfelt ⟨"%5"⟩;dropfelt ⟨"%57"⟩;dropfelt ⟨"%59"⟩;Code.part30;dropfelt ⟨"%4"⟩;dropfelt ⟨"%3"⟩;dropfelt ⟨"%60"⟩;dropfelt ⟨"%62"⟩;Code.part31;dropfelt ⟨"%2"⟩;dropfelt ⟨"%63"⟩;dropfelt ⟨"%65"⟩;dropfelt ⟨"%66"⟩;dropfelt ⟨"%68"⟩;Code.part32;dropfelt ⟨"%1"⟩;dropfelt ⟨"%69"⟩;dropfelt ⟨"%71"⟩;Code.part33;dropfelt ⟨"%20"⟩;dropfelt ⟨"%0"⟩;dropfelt ⟨"%72"⟩;dropfelt ⟨"%74"⟩;dropfelt ⟨"%75"⟩;dropfelt ⟨"%76"⟩;Code.part34;dropfelt ⟨"%78"⟩;dropfelt ⟨"%79"⟩;Code.part35;dropfelt ⟨"%21"⟩;dropfelt ⟨"%77"⟩;dropfelt ⟨"%80"⟩;dropfelt ⟨"%81"⟩;Code.part36;dropfelt ⟨"%22"⟩;dropfelt ⟨"%82"⟩;dropfelt ⟨"%83"⟩;dropfelt ⟨"%84"⟩;Code.part37;dropfelt ⟨"%25"⟩;dropfelt ⟨"%85"⟩;dropfelt ⟨"%86"⟩;dropfelt ⟨"%87"⟩;Code.part38;dropfelt ⟨"%28"⟩;dropfelt ⟨"%88"⟩;dropfelt ⟨"%89"⟩;dropfelt ⟨"%90"⟩;Code.part39;dropfelt ⟨"%31"⟩;dropfelt ⟨"%91"⟩;dropfelt ⟨"%92"⟩;dropfelt ⟨"%93"⟩;Code.part40;dropfelt ⟨"%34"⟩;dropfelt ⟨"%94"⟩;dropfelt ⟨"%95"⟩;dropfelt ⟨"%96"⟩;Code.part41;dropfelt ⟨"%37"⟩;dropfelt ⟨"%97"⟩;dropfelt ⟨"%98"⟩;dropfelt ⟨"%99"⟩;Code.part42;dropfelt ⟨"%40"⟩;dropfelt ⟨"%100"⟩;dropfelt ⟨"%101"⟩;dropfelt ⟨"%102"⟩;Code.part43;dropfelt ⟨"%43"⟩;dropfelt ⟨"%103"⟩;dropfelt ⟨"%104"⟩;dropfelt ⟨"%105"⟩;Code.part44;dropfelt ⟨"%46"⟩;dropfelt ⟨"%106"⟩;dropfelt ⟨"%107"⟩;dropfelt ⟨"%108"⟩;Code.part45;dropfelt ⟨"%49"⟩;dropfelt ⟨"%109"⟩;dropfelt ⟨"%110"⟩;dropfelt ⟨"%111"⟩;Code.part46;dropfelt ⟨"%52"⟩;dropfelt ⟨"%112"⟩;dropfelt ⟨"%113"⟩;dropfelt ⟨"%114"⟩;Code.part47;dropfelt ⟨"%55"⟩;dropfelt ⟨"%115"⟩;dropfelt ⟨"%116"⟩;dropfelt ⟨"%117"⟩;Code.part48;dropfelt ⟨"%58"⟩;dropfelt ⟨"%118"⟩;dropfelt ⟨"%119"⟩;dropfelt ⟨"%120"⟩;Code.part49;dropfelt ⟨"%61"⟩;dropfelt ⟨"%121"⟩;dropfelt ⟨"%122"⟩;dropfelt ⟨"%123"⟩;Code.part50;dropfelt ⟨"%64"⟩;dropfelt ⟨"%124"⟩;dropfelt ⟨"%125"⟩;dropfelt ⟨"%126"⟩;Code.part51;dropfelt ⟨"%67"⟩;dropfelt ⟨"%127"⟩;dropfelt ⟨"%128"⟩;dropfelt ⟨"%129"⟩;Code.part52;dropfelt ⟨"%70"⟩;dropfelt ⟨"%130"⟩;dropfelt ⟨"%131"⟩;dropfelt ⟨"%132"⟩;Code.part53;dropfelt ⟨"%73"⟩;dropfelt ⟨"%133"⟩;dropfelt ⟨"%134"⟩;dropfelt ⟨"%135"⟩;Code.part54;dropfelt ⟨"%18"⟩;dropfelt ⟨"%136"⟩;dropfelt ⟨"%137"⟩;dropfelt ⟨"%19"⟩) = prog
   unfold Code.part16
   MLIR
   rewrite [←eq]
-  rewrite [MLIR.run_seq_def,MLIR.run_dropfelt, MLIR.run_seq_def,MLIR.run_dropfelt, MLIR.run_seq_def,MLIR.run_dropfelt]
+  rewrite [MLIR.run_seq_def,MLIR.run_dropfelt, MLIR.run_seq_def,MLIR.run_dropfelt]
   unfold part16_state_update part16_drops part16_state
   rfl
 
 lemma part16_updates_opaque {st : State} : 
-  Code.getReturn (part15_state_update st) = [y0, y1, y2, y3, y4, y5, y6, y7, y8, y9, y10, y11, y12, y13, y14, y15, y16, y17] ↔
-  Code.getReturn (part16_state_update (part15_drops (part15_state st))) = [y0, y1, y2, y3, y4, y5, y6, y7, y8, y9, y10, y11, y12, y13, y14, y15, y16, y17] := by
+  Code.getReturn (part15_state_update st) = [y0, y1, y2, y3, y4, y5, y6, y7, y8, y9, y10, y11, y12, y13, y14, y15, y16, y17, y18, y19] ↔
+  Code.getReturn (part16_state_update (part15_drops (part15_state st))) = [y0, y1, y2, y3, y4, y5, y6, y7, y8, y9, y10, y11, y12, y13, y14, y15, y16, y17, y18, y19] := by
   simp [part15_state_update, part16_wp]
 
-lemma part16_cumulative_wp {x0 x1 x2 x3: Felt} :
-  Code.run (start_state [x0,x1,x2,x3]) = [y0,y1,y2,y3,y4,y5,y6,y7,y8,y9,y10,y11,y12,y13,y14,y15,y16,y17] ↔
+lemma part16_cumulative_wp {x0: Felt} :
+  Code.run (start_state [x0]) = [y0,y1,y2,y3,y4,y5,y6,y7,y8,y9,y10,y11,y12,y13,y14,y15,y16,y17,y18,y19] ↔
   Code.getReturn
         (part16_state_update
           ({
               buffers :=
-                (Map.empty[{ name := "in" }] ←ₘ [[some x0, some x1, some x2, some x3]])[{ name := "data" }] ←ₘ
-                  [[some (feltBitAnd x3 6 * 1006632961), some (feltBitAnd x3 96 * 1950351361),
-                      some (feltBitAnd x2 96 * 1950351361), some (feltBitAnd x2 3),
-                      some (feltBitAnd x2 12 * 1509949441), some (feltBitAnd x1 48 * 1887436801), none,
-                      some (feltBitAnd x1 12 * 1509949441), some (feltBitAnd x3 8 * 1761607681),
-                      some (feltBitAnd x3 16 * 1887436801), some (feltBitAnd x3 128 * 1997537281),
-                      some (feltBitAnd x2 16 * 1887436801), some (feltBitAnd x2 128 * 1997537281),
-                      some (feltBitAnd x3 1), some (feltBitAnd x1 128 * 1997537281),
-                      some (feltBitAnd x1 64 * 1981808641), none, none]],
-              bufferWidths := ((fun x => Map.empty x)[{ name := "data" }] ←ₘ 18)[{ name := "in" }] ←ₘ 4,
+                (Map.empty[{ name := "code" }] ←ₘ [[some x0]])[{ name := "data" }] ←ₘ
+                  [[some (if x0 = 0 then 1 else 0), some (if x0 - 1 = 0 then 1 else 0),
+                      some (if x0 - 2 = 0 then 1 else 0), some (if x0 - 3 = 0 then 1 else 0),
+                      some (if x0 - 4 = 0 then 1 else 0), some (if x0 - 5 = 0 then 1 else 0),
+                      some (if x0 - 6 = 0 then 1 else 0), some (if x0 - 7 = 0 then 1 else 0),
+                      some (if x0 - 8 = 0 then 1 else 0), some (if x0 - 9 = 0 then 1 else 0),
+                      some (if x0 - 10 = 0 then 1 else 0), some (if x0 - 11 = 0 then 1 else 0),
+                      some (if x0 - 12 = 0 then 1 else 0), some (if x0 - 13 = 0 then 1 else 0),
+                      some (if x0 - 14 = 0 then 1 else 0), some (if x0 - 15 = 0 then 1 else 0), none, none, none,
+                      none]],
+              bufferWidths := ((fun x => Map.empty x)[{ name := "data" }] ←ₘ 20)[{ name := "code" }] ←ₘ 1,
               constraints := [], cycle := 0,
               felts :=
-                (((((((Map.empty[{ name := "%19" }] ←ₘ 128)[{ name := "%23" }] ←ₘ x3)[{ name := "%18" }] ←ₘ
-                            1997537281)[{ name := "%15" }] ←ₘ
-                          16)[{ name := "%13" }] ←ₘ
-                        8)[{ name := "%22" }] ←ₘ
-                      x2)[{ name := "%21" }] ←ₘ
-                    x1)[{ name := "%3" }] ←ₘ
-                  64,
+                (((((((((((((((Map.empty[{ name := "%20" }] ←ₘ x0)[{ name := "%18" }] ←ₘ 1)[{ name := "%17" }] ←ₘ
+                                            2)[{ name := "%16" }] ←ₘ
+                                          3)[{ name := "%15" }] ←ₘ
+                                        4)[{ name := "%14" }] ←ₘ
+                                      5)[{ name := "%13" }] ←ₘ
+                                    6)[{ name := "%12" }] ←ₘ
+                                  7)[{ name := "%11" }] ←ₘ
+                                8)[{ name := "%10" }] ←ₘ
+                              9)[{ name := "%9" }] ←ₘ
+                            10)[{ name := "%8" }] ←ₘ
+                          11)[{ name := "%7" }] ←ₘ
+                        12)[{ name := "%6" }] ←ₘ
+                      13)[{ name := "%5" }] ←ₘ
+                    14)[{ name := "%4" }] ←ₘ
+                  15,
               isFailed := false, props := Map.empty,
-              vars := [{ name := "in" }, { name := "data" }] }[felts][{ name := "%102" }] ←
-            feltBitAnd x1 3)) =
-      [y0, y1, y2, y3, y4, y5, y6, y7, y8, y9, y10, y11, y12, y13, y14, y15, y16, y17]  := by
+              vars := [{ name := "code" }, { name := "data" }] }[felts][{ name := "%3" }] ←
+            16)) =
+      [y0, y1, y2, y3, y4, y5, y6, y7, y8, y9, y10, y11, y12, y13, y14, y15, y16, y17, y18, y19]  := by
     rewrite [part15_cumulative_wp]
     rewrite [part16_updates_opaque]
     unfold part15_state
+    try simplify_get_hack
     MLIR_states_updates
     -- 0 withEqZeros
     -- rewrite [withEqZero_def]
     -- MLIR_states_updates
     unfold part15_drops
-    -- 5 drops
+    -- 2 drops
     simp only [State.drop_update_swap, State.drop_update_same]
     rewrite [State.dropFelts]
     simp only [State.dropFelts_buffers, State.dropFelts_bufferWidths, State.dropFelts_constraints, State.dropFelts_cycle, State.dropFelts_felts, State.dropFelts_isFailed, State.dropFelts_props, State.dropFelts_vars]
