Risc0/Gadgets/OneHot20/Witness/WeakestPresPart29.lean
@@ -10,94 +10,105 @@ open MLIRNotation
 -- The state obtained by running Code.part29 on st
 def part29_state (st: State) : State :=
   
-          ((((st[felts][{ name := "%65" }] ←
-                  Option.get! (State.felts st { name := "%64" }) +
-                    Option.get! (State.felts st { name := "%62" }))[felts][{ name := "%66" }] ←
-                Option.get! (State.felts st { name := "%64" }) + Option.get! (State.felts st { name := "%62" }) +
-                  Option.get! (State.felts st { name := "%57" }))["%55"] ←ₛ
-              getImpl st { name := "data" } 0 6)[felts][{ name := "%67" }] ←
-            Option.get! (State.felts st { name := "%64" }) + Option.get! (State.felts st { name := "%62" }) +
-                Option.get! (State.felts st { name := "%57" }) +
-              Option.get!
-                (State.felts
-                  (((st[felts][{ name := "%65" }] ←
-                        Option.get! (State.felts st { name := "%64" }) +
-                          Option.get! (State.felts st { name := "%62" }))[felts][{ name := "%66" }] ←
-                      Option.get! (State.felts st { name := "%64" }) + Option.get! (State.felts st { name := "%62" }) +
-                        Option.get! (State.felts st { name := "%57" }))["%55"] ←ₛ
-                    getImpl st { name := "data" } 0 6)
-                  { name := "%55" })) 
+          ((((st["%58"] ←ₛ getImpl st { name := "data" } 0 14)[felts][{ name := "%59" }] ←
+                Option.get! (State.felts (st["%58"] ←ₛ getImpl st { name := "data" } 0 14) { name := "%58" }) *
+                  Option.get! (State.felts st { name := "%5" }))[felts][{ name := "%60" }] ←
+              Option.get! (State.felts st { name := "%57" }) +
+                Option.get! (State.felts (st["%58"] ←ₛ getImpl st { name := "data" } 0 14) { name := "%58" }) *
+                  Option.get! (State.felts st { name := "%5" }))["%61"] ←ₛ
+            getImpl st { name := "data" } 0 15) 
 
 def part29_drops (st: State) : State :=
-  State.dropFelts (State.dropFelts (State.dropFelts (State.dropFelts (State.dropFelts (State.dropFelts (st) ⟨"%57"⟩) ⟨"%62"⟩) ⟨"%64"⟩) ⟨"%65"⟩) ⟨"%66"⟩) ⟨"%55"⟩
+  State.dropFelts (State.dropFelts (State.dropFelts (st) ⟨"%5"⟩) ⟨"%57"⟩) ⟨"%59"⟩
 
 -- Run the program from part29 onwards by using part29_state rather than Code.part29
 def part29_state_update (st: State): State :=
-  Γ (part29_drops (part29_state st)) ⟦Code.part30;dropfelt ⟨"%19"⟩;dropfelt ⟨"%21"⟩;dropfelt ⟨"%67"⟩;dropfelt ⟨"%68"⟩;dropfelt ⟨"%70"⟩;Code.part31;dropfelt ⟨"%20"⟩;dropfelt ⟨"%71"⟩;dropfelt ⟨"%69"⟩;dropfelt ⟨"%72"⟩;dropfelt ⟨"%73"⟩⟧
+  Γ (part29_drops (part29_state st)) ⟦Code.part30;dropfelt ⟨"%4"⟩;dropfelt ⟨"%3"⟩;dropfelt ⟨"%60"⟩;dropfelt ⟨"%62"⟩;Code.part31;dropfelt ⟨"%2"⟩;dropfelt ⟨"%63"⟩;dropfelt ⟨"%65"⟩;dropfelt ⟨"%66"⟩;dropfelt ⟨"%68"⟩;Code.part32;dropfelt ⟨"%1"⟩;dropfelt ⟨"%69"⟩;dropfelt ⟨"%71"⟩;Code.part33;dropfelt ⟨"%20"⟩;dropfelt ⟨"%0"⟩;dropfelt ⟨"%72"⟩;dropfelt ⟨"%74"⟩;dropfelt ⟨"%75"⟩;dropfelt ⟨"%76"⟩;Code.part34;dropfelt ⟨"%78"⟩;dropfelt ⟨"%79"⟩;Code.part35;dropfelt ⟨"%21"⟩;dropfelt ⟨"%77"⟩;dropfelt ⟨"%80"⟩;dropfelt ⟨"%81"⟩;Code.part36;dropfelt ⟨"%22"⟩;dropfelt ⟨"%82"⟩;dropfelt ⟨"%83"⟩;dropfelt ⟨"%84"⟩;Code.part37;dropfelt ⟨"%25"⟩;dropfelt ⟨"%85"⟩;dropfelt ⟨"%86"⟩;dropfelt ⟨"%87"⟩;Code.part38;dropfelt ⟨"%28"⟩;dropfelt ⟨"%88"⟩;dropfelt ⟨"%89"⟩;dropfelt ⟨"%90"⟩;Code.part39;dropfelt ⟨"%31"⟩;dropfelt ⟨"%91"⟩;dropfelt ⟨"%92"⟩;dropfelt ⟨"%93"⟩;Code.part40;dropfelt ⟨"%34"⟩;dropfelt ⟨"%94"⟩;dropfelt ⟨"%95"⟩;dropfelt ⟨"%96"⟩;Code.part41;dropfelt ⟨"%37"⟩;dropfelt ⟨"%97"⟩;dropfelt ⟨"%98"⟩;dropfelt ⟨"%99"⟩;Code.part42;dropfelt ⟨"%40"⟩;dropfelt ⟨"%100"⟩;dropfelt ⟨"%101"⟩;dropfelt ⟨"%102"⟩;Code.part43;dropfelt ⟨"%43"⟩;dropfelt ⟨"%103"⟩;dropfelt ⟨"%104"⟩;dropfelt ⟨"%105"⟩;Code.part44;dropfelt ⟨"%46"⟩;dropfelt ⟨"%106"⟩;dropfelt ⟨"%107"⟩;dropfelt ⟨"%108"⟩;Code.part45;dropfelt ⟨"%49"⟩;dropfelt ⟨"%109"⟩;dropfelt ⟨"%110"⟩;dropfelt ⟨"%111"⟩;Code.part46;dropfelt ⟨"%52"⟩;dropfelt ⟨"%112"⟩;dropfelt ⟨"%113"⟩;dropfelt ⟨"%114"⟩;Code.part47;dropfelt ⟨"%55"⟩;dropfelt ⟨"%115"⟩;dropfelt ⟨"%116"⟩;dropfelt ⟨"%117"⟩;Code.part48;dropfelt ⟨"%58"⟩;dropfelt ⟨"%118"⟩;dropfelt ⟨"%119"⟩;dropfelt ⟨"%120"⟩;Code.part49;dropfelt ⟨"%61"⟩;dropfelt ⟨"%121"⟩;dropfelt ⟨"%122"⟩;dropfelt ⟨"%123"⟩;Code.part50;dropfelt ⟨"%64"⟩;dropfelt ⟨"%124"⟩;dropfelt ⟨"%125"⟩;dropfelt ⟨"%126"⟩;Code.part51;dropfelt ⟨"%67"⟩;dropfelt ⟨"%127"⟩;dropfelt ⟨"%128"⟩;dropfelt ⟨"%129"⟩;Code.part52;dropfelt ⟨"%70"⟩;dropfelt ⟨"%130"⟩;dropfelt ⟨"%131"⟩;dropfelt ⟨"%132"⟩;Code.part53;dropfelt ⟨"%73"⟩;dropfelt ⟨"%133"⟩;dropfelt ⟨"%134"⟩;dropfelt ⟨"%135"⟩;Code.part54;dropfelt ⟨"%18"⟩;dropfelt ⟨"%136"⟩;dropfelt ⟨"%137"⟩;dropfelt ⟨"%19"⟩⟧
 
 -- Prove that substituting part29_state for Code.part29 produces the same result
-lemma part29_wp {st : State} {y0 y1 y2 y3 y4 y5 y6 y7 y8 y9 y10 y11 y12 y13 y14 y15 y16 y17 : Option Felt} :
-  Code.getReturn (MLIR.runProgram (Code.part29;dropfelt ⟨"%57"⟩;dropfelt ⟨"%62"⟩;dropfelt ⟨"%64"⟩;dropfelt ⟨"%65"⟩;dropfelt ⟨"%66"⟩;dropfelt ⟨"%55"⟩;Code.part30;dropfelt ⟨"%19"⟩;dropfelt ⟨"%21"⟩;dropfelt ⟨"%67"⟩;dropfelt ⟨"%68"⟩;dropfelt ⟨"%70"⟩;Code.part31;dropfelt ⟨"%20"⟩;dropfelt ⟨"%71"⟩;dropfelt ⟨"%69"⟩;dropfelt ⟨"%72"⟩;dropfelt ⟨"%73"⟩) st) = [y0, y1, y2, y3, y4, y5, y6, y7, y8, y9, y10, y11, y12, y13, y14, y15, y16, y17] ↔
-  Code.getReturn (part29_state_update st) = [y0, y1, y2, y3, y4, y5, y6, y7, y8, y9, y10, y11, y12, y13, y14, y15, y16, y17] := by
+lemma part29_wp {st : State} {y0 y1 y2 y3 y4 y5 y6 y7 y8 y9 y10 y11 y12 y13 y14 y15 y16 y17 y18 y19 : Option Felt} :
+  Code.getReturn (MLIR.runProgram (Code.part29;dropfelt ⟨"%5"⟩;dropfelt ⟨"%57"⟩;dropfelt ⟨"%59"⟩;Code.part30;dropfelt ⟨"%4"⟩;dropfelt ⟨"%3"⟩;dropfelt ⟨"%60"⟩;dropfelt ⟨"%62"⟩;Code.part31;dropfelt ⟨"%2"⟩;dropfelt ⟨"%63"⟩;dropfelt ⟨"%65"⟩;dropfelt ⟨"%66"⟩;dropfelt ⟨"%68"⟩;Code.part32;dropfelt ⟨"%1"⟩;dropfelt ⟨"%69"⟩;dropfelt ⟨"%71"⟩;Code.part33;dropfelt ⟨"%20"⟩;dropfelt ⟨"%0"⟩;dropfelt ⟨"%72"⟩;dropfelt ⟨"%74"⟩;dropfelt ⟨"%75"⟩;dropfelt ⟨"%76"⟩;Code.part34;dropfelt ⟨"%78"⟩;dropfelt ⟨"%79"⟩;Code.part35;dropfelt ⟨"%21"⟩;dropfelt ⟨"%77"⟩;dropfelt ⟨"%80"⟩;dropfelt ⟨"%81"⟩;Code.part36;dropfelt ⟨"%22"⟩;dropfelt ⟨"%82"⟩;dropfelt ⟨"%83"⟩;dropfelt ⟨"%84"⟩;Code.part37;dropfelt ⟨"%25"⟩;dropfelt ⟨"%85"⟩;dropfelt ⟨"%86"⟩;dropfelt ⟨"%87"⟩;Code.part38;dropfelt ⟨"%28"⟩;dropfelt ⟨"%88"⟩;dropfelt ⟨"%89"⟩;dropfelt ⟨"%90"⟩;Code.part39;dropfelt ⟨"%31"⟩;dropfelt ⟨"%91"⟩;dropfelt ⟨"%92"⟩;dropfelt ⟨"%93"⟩;Code.part40;dropfelt ⟨"%34"⟩;dropfelt ⟨"%94"⟩;dropfelt ⟨"%95"⟩;dropfelt ⟨"%96"⟩;Code.part41;dropfelt ⟨"%37"⟩;dropfelt ⟨"%97"⟩;dropfelt ⟨"%98"⟩;dropfelt ⟨"%99"⟩;Code.part42;dropfelt ⟨"%40"⟩;dropfelt ⟨"%100"⟩;dropfelt ⟨"%101"⟩;dropfelt ⟨"%102"⟩;Code.part43;dropfelt ⟨"%43"⟩;dropfelt ⟨"%103"⟩;dropfelt ⟨"%104"⟩;dropfelt ⟨"%105"⟩;Code.part44;dropfelt ⟨"%46"⟩;dropfelt ⟨"%106"⟩;dropfelt ⟨"%107"⟩;dropfelt ⟨"%108"⟩;Code.part45;dropfelt ⟨"%49"⟩;dropfelt ⟨"%109"⟩;dropfelt ⟨"%110"⟩;dropfelt ⟨"%111"⟩;Code.part46;dropfelt ⟨"%52"⟩;dropfelt ⟨"%112"⟩;dropfelt ⟨"%113"⟩;dropfelt ⟨"%114"⟩;Code.part47;dropfelt ⟨"%55"⟩;dropfelt ⟨"%115"⟩;dropfelt ⟨"%116"⟩;dropfelt ⟨"%117"⟩;Code.part48;dropfelt ⟨"%58"⟩;dropfelt ⟨"%118"⟩;dropfelt ⟨"%119"⟩;dropfelt ⟨"%120"⟩;Code.part49;dropfelt ⟨"%61"⟩;dropfelt ⟨"%121"⟩;dropfelt ⟨"%122"⟩;dropfelt ⟨"%123"⟩;Code.part50;dropfelt ⟨"%64"⟩;dropfelt ⟨"%124"⟩;dropfelt ⟨"%125"⟩;dropfelt ⟨"%126"⟩;Code.part51;dropfelt ⟨"%67"⟩;dropfelt ⟨"%127"⟩;dropfelt ⟨"%128"⟩;dropfelt ⟨"%129"⟩;Code.part52;dropfelt ⟨"%70"⟩;dropfelt ⟨"%130"⟩;dropfelt ⟨"%131"⟩;dropfelt ⟨"%132"⟩;Code.part53;dropfelt ⟨"%73"⟩;dropfelt ⟨"%133"⟩;dropfelt ⟨"%134"⟩;dropfelt ⟨"%135"⟩;Code.part54;dropfelt ⟨"%18"⟩;dropfelt ⟨"%136"⟩;dropfelt ⟨"%137"⟩;dropfelt ⟨"%19"⟩) st) = [y0, y1, y2, y3, y4, y5, y6, y7, y8, y9, y10, y11, y12, y13, y14, y15, y16, y17, y18, y19] ↔
+  Code.getReturn (part29_state_update st) = [y0, y1, y2, y3, y4, y5, y6, y7, y8, y9, y10, y11, y12, y13, y14, y15, y16, y17, y18, y19] := by
   unfold MLIR.runProgram; simp only
-  generalize eq : (dropfelt ⟨"%57"⟩;dropfelt ⟨"%62"⟩;dropfelt ⟨"%64"⟩;dropfelt ⟨"%65"⟩;dropfelt ⟨"%66"⟩;dropfelt ⟨"%55"⟩;Code.part30;dropfelt ⟨"%19"⟩;dropfelt ⟨"%21"⟩;dropfelt ⟨"%67"⟩;dropfelt ⟨"%68"⟩;dropfelt ⟨"%70"⟩;Code.part31;dropfelt ⟨"%20"⟩;dropfelt ⟨"%71"⟩;dropfelt ⟨"%69"⟩;dropfelt ⟨"%72"⟩;dropfelt ⟨"%73"⟩) = prog
+  generalize eq : (dropfelt ⟨"%5"⟩;dropfelt ⟨"%57"⟩;dropfelt ⟨"%59"⟩;Code.part30;dropfelt ⟨"%4"⟩;dropfelt ⟨"%3"⟩;dropfelt ⟨"%60"⟩;dropfelt ⟨"%62"⟩;Code.part31;dropfelt ⟨"%2"⟩;dropfelt ⟨"%63"⟩;dropfelt ⟨"%65"⟩;dropfelt ⟨"%66"⟩;dropfelt ⟨"%68"⟩;Code.part32;dropfelt ⟨"%1"⟩;dropfelt ⟨"%69"⟩;dropfelt ⟨"%71"⟩;Code.part33;dropfelt ⟨"%20"⟩;dropfelt ⟨"%0"⟩;dropfelt ⟨"%72"⟩;dropfelt ⟨"%74"⟩;dropfelt ⟨"%75"⟩;dropfelt ⟨"%76"⟩;Code.part34;dropfelt ⟨"%78"⟩;dropfelt ⟨"%79"⟩;Code.part35;dropfelt ⟨"%21"⟩;dropfelt ⟨"%77"⟩;dropfelt ⟨"%80"⟩;dropfelt ⟨"%81"⟩;Code.part36;dropfelt ⟨"%22"⟩;dropfelt ⟨"%82"⟩;dropfelt ⟨"%83"⟩;dropfelt ⟨"%84"⟩;Code.part37;dropfelt ⟨"%25"⟩;dropfelt ⟨"%85"⟩;dropfelt ⟨"%86"⟩;dropfelt ⟨"%87"⟩;Code.part38;dropfelt ⟨"%28"⟩;dropfelt ⟨"%88"⟩;dropfelt ⟨"%89"⟩;dropfelt ⟨"%90"⟩;Code.part39;dropfelt ⟨"%31"⟩;dropfelt ⟨"%91"⟩;dropfelt ⟨"%92"⟩;dropfelt ⟨"%93"⟩;Code.part40;dropfelt ⟨"%34"⟩;dropfelt ⟨"%94"⟩;dropfelt ⟨"%95"⟩;dropfelt ⟨"%96"⟩;Code.part41;dropfelt ⟨"%37"⟩;dropfelt ⟨"%97"⟩;dropfelt ⟨"%98"⟩;dropfelt ⟨"%99"⟩;Code.part42;dropfelt ⟨"%40"⟩;dropfelt ⟨"%100"⟩;dropfelt ⟨"%101"⟩;dropfelt ⟨"%102"⟩;Code.part43;dropfelt ⟨"%43"⟩;dropfelt ⟨"%103"⟩;dropfelt ⟨"%104"⟩;dropfelt ⟨"%105"⟩;Code.part44;dropfelt ⟨"%46"⟩;dropfelt ⟨"%106"⟩;dropfelt ⟨"%107"⟩;dropfelt ⟨"%108"⟩;Code.part45;dropfelt ⟨"%49"⟩;dropfelt ⟨"%109"⟩;dropfelt ⟨"%110"⟩;dropfelt ⟨"%111"⟩;Code.part46;dropfelt ⟨"%52"⟩;dropfelt ⟨"%112"⟩;dropfelt ⟨"%113"⟩;dropfelt ⟨"%114"⟩;Code.part47;dropfelt ⟨"%55"⟩;dropfelt ⟨"%115"⟩;dropfelt ⟨"%116"⟩;dropfelt ⟨"%117"⟩;Code.part48;dropfelt ⟨"%58"⟩;dropfelt ⟨"%118"⟩;dropfelt ⟨"%119"⟩;dropfelt ⟨"%120"⟩;Code.part49;dropfelt ⟨"%61"⟩;dropfelt ⟨"%121"⟩;dropfelt ⟨"%122"⟩;dropfelt ⟨"%123"⟩;Code.part50;dropfelt ⟨"%64"⟩;dropfelt ⟨"%124"⟩;dropfelt ⟨"%125"⟩;dropfelt ⟨"%126"⟩;Code.part51;dropfelt ⟨"%67"⟩;dropfelt ⟨"%127"⟩;dropfelt ⟨"%128"⟩;dropfelt ⟨"%129"⟩;Code.part52;dropfelt ⟨"%70"⟩;dropfelt ⟨"%130"⟩;dropfelt ⟨"%131"⟩;dropfelt ⟨"%132"⟩;Code.part53;dropfelt ⟨"%73"⟩;dropfelt ⟨"%133"⟩;dropfelt ⟨"%134"⟩;dropfelt ⟨"%135"⟩;Code.part54;dropfelt ⟨"%18"⟩;dropfelt ⟨"%136"⟩;dropfelt ⟨"%137"⟩;dropfelt ⟨"%19"⟩) = prog
   unfold Code.part29
   MLIR
   rewrite [←eq]
-  rewrite [MLIR.run_seq_def,MLIR.run_dropfelt, MLIR.run_seq_def,MLIR.run_dropfelt, MLIR.run_seq_def,MLIR.run_dropfelt, MLIR.run_seq_def,MLIR.run_dropfelt, MLIR.run_seq_def,MLIR.run_dropfelt, MLIR.run_seq_def,MLIR.run_dropfelt]
+  rewrite [MLIR.run_seq_def,MLIR.run_dropfelt, MLIR.run_seq_def,MLIR.run_dropfelt, MLIR.run_seq_def,MLIR.run_dropfelt]
   unfold part29_state_update part29_drops part29_state
   rfl
 
 lemma part29_updates_opaque {st : State} : 
-  Code.getReturn (part28_state_update st) = [y0, y1, y2, y3, y4, y5, y6, y7, y8, y9, y10, y11, y12, y13, y14, y15, y16, y17] ↔
-  Code.getReturn (part29_state_update (part28_drops (part28_state st))) = [y0, y1, y2, y3, y4, y5, y6, y7, y8, y9, y10, y11, y12, y13, y14, y15, y16, y17] := by
+  Code.getReturn (part28_state_update st) = [y0, y1, y2, y3, y4, y5, y6, y7, y8, y9, y10, y11, y12, y13, y14, y15, y16, y17, y18, y19] ↔
+  Code.getReturn (part29_state_update (part28_drops (part28_state st))) = [y0, y1, y2, y3, y4, y5, y6, y7, y8, y9, y10, y11, y12, y13, y14, y15, y16, y17, y18, y19] := by
   simp [part28_state_update, part29_wp]
 
-lemma part29_cumulative_wp {x0 x1 x2 x3: Felt} :
-  Code.run (start_state [x0,x1,x2,x3]) = [y0,y1,y2,y3,y4,y5,y6,y7,y8,y9,y10,y11,y12,y13,y14,y15,y16,y17] ↔
+lemma part29_cumulative_wp {x0: Felt} :
+  Code.run (start_state [x0]) = [y0,y1,y2,y3,y4,y5,y6,y7,y8,y9,y10,y11,y12,y13,y14,y15,y16,y17,y18,y19] ↔
   Code.getReturn
         (part29_state_update
-          ((({
-                  buffers :=
-                    ((fun x => Map.empty x)[{ name := "in" }] ←ₘ
-                        [[some x0, some x1, some x2, some x3]])[{ name := "data" }] ←ₘ
-                      [[some (feltBitAnd x3 6 * 1006632961), some (feltBitAnd x3 96 * 1950351361),
-                          some (feltBitAnd x2 96 * 1950351361), some (feltBitAnd x2 3),
-                          some (feltBitAnd x2 12 * 1509949441), some (feltBitAnd x1 48 * 1887436801),
-                          some (feltBitAnd x1 3), some (feltBitAnd x1 12 * 1509949441),
-                          some (feltBitAnd x3 8 * 1761607681), some (feltBitAnd x3 16 * 1887436801),
-                          some (feltBitAnd x3 128 * 1997537281), some (feltBitAnd x2 16 * 1887436801),
-                          some (feltBitAnd x2 128 * 1997537281), some (feltBitAnd x3 1),
-                          some (feltBitAnd x1 128 * 1997537281), some (feltBitAnd x1 64 * 1981808641),
-                          some (feltBitAnd x0 128 * 1997537281), some (feltBitAnd x0 127)]],
-                  bufferWidths := ((fun x => Map.empty x)[{ name := "data" }] ←ₘ 18)[{ name := "in" }] ←ₘ 4,
-                  constraints :=
-                    [x2 -
-                          ((feltBitAnd x2 128 * 1997537281 * 8 + feltBitAnd x2 96 * 1950351361 * 2 +
-                                  feltBitAnd x2 16 * 1887436801) *
-                                16 +
-                              feltBitAnd x2 12 * 1509949441 * 4 +
-                            feltBitAnd x2 3) =
-                        0,
-                      x3 -
-                          ((feltBitAnd x3 128 * 1997537281 * 64 +
-                                (feltBitAnd x3 96 * 1950351361 * 16 + feltBitAnd x3 16 * 1887436801 * 8 +
-                                    feltBitAnd x3 8 * 1761607681 * 4 +
-                                  feltBitAnd x3 6 * 1006632961)) *
-                              2 +
-                            feltBitAnd x3 1) =
-                        0],
-                  cycle := 0,
-                  felts := ((Map.empty[{ name := "%19" }] ←ₘ 128)[{ name := "%21" }] ←ₘ x1)[{ name := "%20" }] ←ₘ x0,
-                  isFailed := false, props := Map.empty,
-                  vars := [{ name := "in" }, { name := "data" }] }[felts][{ name := "%57" }] ←
-                feltBitAnd x1 12 * 1509949441 * 4)[felts][{ name := "%62" }] ←
-              (feltBitAnd x1 64 * 1981808641 * 4 + feltBitAnd x1 48 * 1887436801) * 16)[felts][{ name := "%64" }] ←
-            feltBitAnd x1 128 * 1997537281 * 128)) =
-      [y0, y1, y2, y3, y4, y5, y6, y7, y8, y9, y10, y11, y12, y13, y14, y15, y16, y17]  := by
+          (((((((((((((({
+                                        buffers :=
+                                          ((fun x => Map.empty x)[{ name := "code" }] ←ₘ
+                                              [[some x0]])[{ name := "data" }] ←ₘ
+                                            [[some (if x0 = 0 then 1 else 0), some (if x0 - 1 = 0 then 1 else 0),
+                                                some (if x0 - 2 = 0 then 1 else 0), some (if x0 - 3 = 0 then 1 else 0),
+                                                some (if x0 - 4 = 0 then 1 else 0), some (if x0 - 5 = 0 then 1 else 0),
+                                                some (if x0 - 6 = 0 then 1 else 0), some (if x0 - 7 = 0 then 1 else 0),
+                                                some (if x0 - 8 = 0 then 1 else 0), some (if x0 - 9 = 0 then 1 else 0),
+                                                some (if x0 - 10 = 0 then 1 else 0),
+                                                some (if x0 - 11 = 0 then 1 else 0),
+                                                some (if x0 - 12 = 0 then 1 else 0),
+                                                some (if x0 - 13 = 0 then 1 else 0),
+                                                some (if x0 - 14 = 0 then 1 else 0),
+                                                some (if x0 - 15 = 0 then 1 else 0),
+                                                some (if x0 - 16 = 0 then 1 else 0),
+                                                some (if x0 - 17 = 0 then 1 else 0),
+                                                some (if x0 - 18 = 0 then 1 else 0),
+                                                some (if x0 - 19 = 0 then 1 else 0)]],
+                                        bufferWidths :=
+                                          ((fun x => Map.empty x)[{ name := "data" }] ←ₘ 20)[{ name := "code" }] ←ₘ 1,
+                                        constraints := [], cycle := 0,
+                                        felts :=
+                                          (((((((Map.empty[{ name := "%20" }] ←ₘ x0)[{ name := "%18" }] ←ₘ
+                                                        1)[{ name := "%5" }] ←ₘ
+                                                      14)[{ name := "%4" }] ←ₘ
+                                                    15)[{ name := "%3" }] ←ₘ
+                                                  16)[{ name := "%2" }] ←ₘ
+                                                17)[{ name := "%1" }] ←ₘ
+                                              18)[{ name := "%0" }] ←ₘ
+                                            19,
+                                        isFailed := false, props := Map.empty,
+                                        vars := [{ name := "code" }, { name := "data" }] }[felts][{ name := "%22" }] ←
+                                      if x0 - 2 = 0 then 1 else 0)[felts][{ name := "%21" }] ←
+                                    if x0 - 1 = 0 then 1 else 0)[felts][{ name := "%25" }] ←
+                                  if x0 - 3 = 0 then 1 else 0)[felts][{ name := "%28" }] ←
+                                if x0 - 4 = 0 then 1 else 0)[felts][{ name := "%31" }] ←
+                              if x0 - 5 = 0 then 1 else 0)[felts][{ name := "%34" }] ←
+                            if x0 - 6 = 0 then 1 else 0)[felts][{ name := "%37" }] ←
+                          if x0 - 7 = 0 then 1 else 0)[felts][{ name := "%40" }] ←
+                        if x0 - 8 = 0 then 1 else 0)[felts][{ name := "%43" }] ←
+                      if x0 - 9 = 0 then 1 else 0)[felts][{ name := "%46" }] ←
+                    if x0 - 10 = 0 then 1 else 0)[felts][{ name := "%49" }] ←
+                  if x0 - 11 = 0 then 1 else 0)[felts][{ name := "%52" }] ←
+                if x0 - 12 = 0 then 1 else 0)[felts][{ name := "%55" }] ←
+              if x0 - 13 = 0 then 1 else 0)[felts][{ name := "%57" }] ←
+            (if x0 - 1 = 0 then 1 else 0) + (if x0 - 2 = 0 then 1 else 0) * 2 + (if x0 - 3 = 0 then 1 else 0) * 3 +
+                                (if x0 - 4 = 0 then 1 else 0) * 4 +
+                              (if x0 - 5 = 0 then 1 else 0) * 5 +
+                            (if x0 - 6 = 0 then 1 else 0) * 6 +
+                          (if x0 - 7 = 0 then 1 else 0) * 7 +
+                        (if x0 - 8 = 0 then 1 else 0) * 8 +
+                      (if x0 - 9 = 0 then 1 else 0) * 9 +
+                    (if x0 - 10 = 0 then 1 else 0) * 10 +
+                  (if x0 - 11 = 0 then 1 else 0) * 11 +
+                (if x0 - 12 = 0 then 1 else 0) * 12 +
+              (if x0 - 13 = 0 then 1 else 0) * 13)) =
+      [y0, y1, y2, y3, y4, y5, y6, y7, y8, y9, y10, y11, y12, y13, y14, y15, y16, y17, y18, y19]  := by
     rewrite [part28_cumulative_wp]
     rewrite [part29_updates_opaque]
     unfold part28_state
+    try simplify_get_hack
     MLIR_states_updates
     -- 0 withEqZeros
     -- rewrite [withEqZero_def]
